add and use more utils

AdventOfCode/Utils.lean
@@ -1,3 +1,89 @@
 export Function (curry uncurry)
 
 def dup (f : α -> α -> β) (x : α) := f x x
+
+namespace Nat
+
+  def addInt (lhs : Nat) : Int -> Nat
+  | .ofNat rhs => lhs + rhs
+  | .negSucc rhs => lhs - rhs.succ
+
+  def maxInt (lhs : Nat) : Int -> Nat
+  | .ofNat rhs => max lhs rhs
+  | .negSucc _ => lhs
+
+  def diff (lhs rhs : Nat) :=
+    Int.ofNat lhs - Int.ofNat rhs
+
+end Nat
+
+namespace Std
+
+  instance (i : Nat) (r : Range) : Decidable (i ∈ r) := by
+    unfold Membership.mem
+    unfold instMembershipNatRange
+    infer_instance
+
+  example : 0 ∈ [:1] := by decide
+  example : 0 ∈ [0:1] := by decide
+  example : 0 ∈ [0:1:1] := by decide
+  example : 0 ∈ [:1:1] := by decide
+
+end Std
+
+namespace StreamRange
+
+  structure StreamRange where
+    start : Nat := 0
+    step : Nat := 1
+
+  instance : Membership Nat StreamRange where
+    mem r i := if r.start + r.step >= r.start then r.start <= i else r.start >= i
+
+  instance (i : Nat) (r : StreamRange) : Decidable (i ∈ r) := by
+    unfold Membership.mem
+    unfold instMembershipNatStreamRange
+    infer_instance
+
+  instance : ForIn m StreamRange Nat where
+    forIn x b f := do
+      let mut i := x.start
+      let mut b := b
+      while true do
+        match (<- f i b) with
+        | .yield b' => do
+          b := b'
+          i := i + x.step
+        | .done b' => do
+          b := b'
+          break
+        i := i + x.step
+      return b
+
+  syntax:max "[" withoutPosition(":") "]" : term
+  syntax:max "[" withoutPosition(term ":") "]" : term
+  syntax:max "[" withoutPosition(":" ":" term) "]" : term
+  syntax:max "[" withoutPosition("::" term) "]" : term
+  syntax:max "[" withoutPosition(term ":" ":" term) "]" : term
+  syntax:max "[" withoutPosition(term "::" term) "]" : term
+
+  macro_rules
+  | `([:]) => `({ start := 0, step := 1 : StreamRange })
+  | `([ $start :]) => `({ start := $start, step := 1 : StreamRange })
+  | `([: : $step ]) => `({ start := 0, step := $step : StreamRange })
+  | `([:: $step ]) => `({ start := 0, step := $step : StreamRange })
+  | `([ $start : : $step ]) => `({ start := $start, step := $step : StreamRange })
+  | `([ $start :: $step ]) => `({ start := $start, step := $step : StreamRange })
+
+  example : 0 ∈ [:] := by decide
+  example : 0 ∈ [::1] := by decide
+  example : 0 ∈ [0:] := by decide
+  example : 0 ∈ [0::1] := by decide
+
+  instance : Stream StreamRange Nat where
+    next? range := (range.start, { range with start := range.start + range.step })
+
+  instance : ToStream StreamRange StreamRange where
+    toStream range := range
+
+end StreamRange
