AdventOfCode/Day2.lean
@@ -8,7 +8,7 @@ def parseInput (input : String) :=
 
 def checkDiff (diff : List Int) :=
   (diff.all (· > 0) || diff.all (· < 0)) &&
-  diff.all (·.natAbs |> dup (· >= 1 && · <= 3))
+  diff.all (·.natAbs |> (· ∈ [1:4]))
 
 def solvePart1 (input : List (List Nat)) :=
   input.countP fun report =>
